\documentclass[12pt]{exam}
\usepackage[utf8]{inputenc}
\usepackage{amsmath}
\usepackage{amssymb}
\usepackage{tabto}

\title{\textbf{MATH 311 Homework 2.3}}
\author{Will Townsend}
\date{February 14, 2022}

\begin{document}

\maketitle

\section*{Problem 7}
\large\begin{eqnarray*}
    x\dfrac{dy}{dx}=y^{-3}=>y^3dy=x^{-1}dx=>\int y^3dy=\int x^{-1}dx\\\\
    \dfrac{y^4}{4}=\ln{x}+C=>y^4=4\ln{x}+C
\end{eqnarray*}
\section*{Problem 8}
\large\begin{eqnarray*}
    \dfrac{dx}{dt}=3xt^2=>\int\dfrac{dx}{3x}=\int t^2dt=>
    \dfrac{\ln{|3x|}}{3}=\dfrac{t^3}{3}+C\\\\
    =>x=e^{\frac{t^3}{3}+C}=>x=Ae^{\frac{t^3}{3}}
\end{eqnarray*}
\section*{Problem 9}
\large\begin{eqnarray*}
    \dfrac{dx}{dt}=\dfrac{t}{xe^{t+2x}}=>e^{t+2x}dx=\dfrac{t}{x}dt
    =>t+2x\:dx=\ln{t}-\ln{x}\:dt=>\\\\
    \int 2x+\ln{x}\:dx=\int\ln{t}-t\:dt=>x^2+x\ln{x}-x=t\ln{t}-t-\dfrac{t^2}{2}+C
\end{eqnarray*}
\pagebreak
\section*{Problem 10}
\large\begin{eqnarray*}
    \dfrac{dy}{dx}=\dfrac{x}{y^2\sqrt{x+1}}=>\int y^2\:dy= \int\dfrac{x}{\sqrt{x+1}}\:dx=>\dfrac{y^3}{3}= \dfrac{2(x+1)^\frac{3}{2}}{3}-2\sqrt{x+1}+C\\\\
    y^3=2(x+1)^\frac{3}{2}-6\sqrt{x+1}+C
\end{eqnarray*}
Integration (using u sub where $u=x+1\quad du=dx$):
\large\begin{eqnarray*}
    \int\dfrac{x}{\sqrt{x+1}}\:dx=\int\dfrac{u-1}{\sqrt{u}}\:du
    =\int\sqrt{u}-(u)^{-\frac{1}{2}}du=>\dfrac{2(x+1)^\frac{3}{2}}{3}-2\sqrt{x+1}+C\\
\end{eqnarray*}
\section*{Problem 13}
\large\begin{eqnarray*}
    \dfrac{dy}{dx}=3x^2(1+y^2)^\frac{3}{2}=>\int(1+y^2)^{-\frac{3}{2}}\:dy=\int3x^2\:dx=>\dfrac{y}{\sqrt{y^2+1}}=x^3+C
\end{eqnarray*}
Integration (using trig sub $y=\tan{\theta}$):
\large\begin{eqnarray*}
    \int\dfrac{dy}{\sqrt{(y^2+1)^3}}=\int\dfrac{\sec^2{\theta}}{\sec^3\theta}\:d\theta=\int\cos{\theta}\:d\theta=\sin{\theta}+C=\dfrac{y}{\sqrt{y^2+1}}+C\\
\end{eqnarray*}
\section*{Problem 14}
\large\begin{eqnarray*}
    \dfrac{dx}{dt}-x^3=x=>\dfrac{dx}{dt}=x^3+x=>\int\dfrac{dx}{x^3+x}=\int dt=>\\\\
    \ln{\left(\dfrac{|x|}{\sqrt{x^2+1}}\right)}=t+C=>\dfrac{|x|}{\sqrt{x^2+1}}=Ae^t
\end{eqnarray*}
Integration (using partial fractions):
\large\begin{eqnarray*}
    \int\dfrac{dx}{x^3+x}=\int\dfrac{A}{x}+\dfrac{Bx+C}{x^2+1}\:dx=\int\dfrac{1}{x}-\dfrac{x}{x^2+1}dx=\ln{\left(\dfrac{|x|}{\sqrt{x^2+1}}\right)}+C
\end{eqnarray*}
\section*{Problem 15}
\large\begin{eqnarray*}
    (x+xy^2)\:dx+e^{x^2}y\:dy=0=>\dfrac{(1+y^2)}{y}dx=-\dfrac{e^{x^2}}{x}dy=>\\\\
    \int-\dfrac{x}{e^{x^2}}\:dx=\int\dfrac{y}{1+y^2}\:dy=>\dfrac{e^{-x^2}}{2}+C=\ln{\left(\sqrt{y^2+1}\right)}=>\\\\
    e^{\frac{e^{-x^2}}{2}}+C=\sqrt{y^2+1}
\end{eqnarray*}
Integration (simple u subs)
\section*{Problem 16}
\large\begin{eqnarray*}
    y^{-1}\:dy+ye^{\cos{x}}\sin{x}\:dx=0=>-y^{-2}\:dy=e^{\cos{x}}\sin{x}\:dx=>\\\\
    \int-2\ln{y}\:dy=\int\cos{x}\ln{(\sin{x})}\:dx=>-y\ln{y}+y=\sin{x}\ln{(\sin{x})}-\sin{x}+C\\
\end{eqnarray*}
Integration (u sub)
\section*{Problem 17}
\begin{center}$\dfrac{dy}{dx}=(1+y^2)\tan{x}\qquad y(0)=\sqrt{3}$\end{center}
\large\begin{eqnarray*}
    \int(1+y^2)^{-1}\:dy=\int\tan{x}\:dx=>\tan^{-1}{y}=\ln{|\cos{x}|}+C
\end{eqnarray*}
Find $C$:\\\\
$\tan^{-1}{0}=\ln{|\cos{\sqrt{2}}|}+C=>C=-\ln{|\cos{\sqrt{2}}|}$\\\\
Final Solution:\\\\
$\tan^{-1}{y}=\ln{|\cos{x}|}-\ln{|\cos{\sqrt{2}}|}=>y=\ln{\left(\dfrac{|\cos{x}|}{|\cos{\sqrt{2}}|}\right)}$
\section*{Problem 18}
\begin{center}$y'=x^3(1-y) \qquad y(0)=3$\end{center}
\large\begin{eqnarray*}
    \int\dfrac{1}{1-y}\:dy=\int x^3\:dx=>-\ln{|1-y|}=\dfrac{x^4}{4}+C=>(1-y)^{-1}=Ae^{\frac{x^4}{4}}
\end{eqnarray*}
Find A:\\\\
$(1-3)^{-1}=Ae^{\frac{0^4}{4}}=>-\frac{1}{2}=A$\\\\
Final Solution:\\\\
$(1-y)^{-1}=-\frac{1}{2}e^{\frac{x^4}{4}}$
\section*{Problem 19}
\begin{center}$\frac{1}{2}\frac{dy}{dx}=\sqrt{y+1}\cos{x} \qquad y(\pi)=0$\end{center}
\large\begin{eqnarray*}
    \dfrac{1}{2}\int\dfrac{1}{\sqrt{y+1}}\:dy=\int\cos{x}\:dx=>\sqrt{y+1}=\sin{x}+C
\end{eqnarray*}
Find $C$:\\\\
$\sqrt{0+1}=\sin{\pi}+C=>C=1$\\\\
Final Solution:\\\\
$\sqrt{y+1}=\sin{x}+1$
\pagebreak
\section*{Problem 20}
\begin{center}$x^2\dfrac{dy}{dx}=\dfrac{4x^2-x-2}{(x+1)(y+1)}\qquad y(1)=1$\end{center}
\large\begin{eqnarray*}
    \int y+1\:dy=\int\dfrac{4x^2-x-2}{x^2(x+1)}\:dx=>\frac{1}{2}y^2+y=\dfrac{2}{x}+\ln{|x|}+3\ln{|x+1|}+C
\end{eqnarray*}\\
Find $C$:\\\\
$\frac{3}{2}=2+0+3\ln{2}+C=>C=-\ln{8}-\frac{1}{2}$\\\\
Final Solution:\\\\
$\frac{1}{2}y^2+y=\dfrac{2}{x}+\ln{|x|}+3\ln{|x+1|}-\ln{8}-\frac{1}{2}$
\section*{Problem 34}
\begin{center}$\dfrac{dT}{dt}=k(M-T)$\end{center}
\large\begin{eqnarray*}
    \int(M-T)^{-1}\:dT=\int k\:dt=>\ln{\left[(M-T)^{-1}\right]}=kt+C=>M-T=
    Ae^{-kt}
\end{eqnarray*}\\
$T(t)=M-Ae^{-kt}$\\\\
$T(0)=100=>100=70-A=>A=-30$\\\\
$T(6)=80=>80=70+30e^{-6k}=>\dfrac{1}{3}=e^{-6k}=>-\ln{(3)}=\dfrac{1}{6k}=>$\\\\
$k=-\dfrac{1}{6\ln{(3)}}$\\\\
$T(20)=70+30e^{-\frac{10}{3\ln{(3)}}}\approx71.44^{\circ}F$
\section*{Problem 35}
Find our constants:\\\\
$40=120-A=>A=80$\\\\
$90=120-80e^{-45k}=>\ln{\left(\dfrac{3}{8}\right)}=-45k=>k=-\dfrac{\ln{\left(\dfrac{3}{8}\right)}}{45}$\\\\
Part A ($M=100$):\\\\
$90=100-80e^{\frac{t\ln{\left(\frac{3}{8}\right)}}{45}}=>\frac{1}{8}=e^{\frac{t\ln{\left(\frac{3}{8}\right)}}{45}}=>t=45\ln{\frac{1}{8}}(\ln{\frac{3}{8}})^{-1}\approx95.40$ min\\\\
Part B ($M=140$):\\\\
$90=140-80e^{\frac{t\ln{\left(\frac{3}{8}\right)}}{45}}=>\frac{5}{8}=e^{\frac{t\ln{\left(\frac{3}{8}\right)}}{45}}=>t=45\ln{\frac{5}{8}}(\ln{\frac{3}{8}})^{-1}\approx21.56$ min\\\\
Part C ($M=80$):\\\\
$90=80-80e^{\frac{t\ln{\left(\frac{3}{8}\right)}}{45}}=>-\frac{1}{8}=e^{\frac{t\ln{\left(\frac{3}{8}\right)}}{45}}$ (Solution Impossible to find)
\end{document}
