\documentclass[12pt]{exam}
\usepackage[utf8]{inputenc}
\usepackage{amsmath}
\usepackage{amssymb}
\usepackage{tabto}

\title{Homework 1}
\author{Will Townsend}
\date{February 8, 2022}

\begin{document}

\maketitle

\begin{center}\Large{\textbf{\underline{Chapter 1.1}}}\end{center}
1. Second order, Linear ODE Dependent=$x$ Independent=$t$\\\\
2. Second order, Linear ODE Dependent=$y$ Independent=$x$\\\\
3. First order, Non-Linear ODE Dependent=$y$ Independent=$x$\\\\
4. Second order, Linear PDE Dependent=$u$ Independent=$x,y$\\\\
5. First order, Non-Linear ODE Dependent=$y$ Independent=$x$\\\\
6. First order, Non-Linear ODE Dependent=$x$ Independent=$t$\\\\
7. First order, Non-Linear ODE Dependent=$p$ Independent=$t$\\\\
8. Second order, Non-Linear ODE Dependent=$y$ Independent=$x$\\\\
9. Second order, Linear, ODE Dependent=$y$ Independent=$x$\\\\
10. Fourth order, Linear ODE Dependent=$y$ Independent=$x$\\\\
11. Second order, Linear PDE Dependent=$N$ Independent=$r$\\\\
12. Second order, Non-Linear ODE Dependent=$y$ Independent=$x$\\

\pagebreak

\begin{center}\Large{\textbf{\underline{Chapter1.2}}}\end{center}
Problem 3:\\\\$y=\sin{x}+x^2$ \tab{$\dfrac{d^2y}{dx^2}+y=x^2+2$}\\\\
$y'=\cos{x}+2x$ \tab{$y''=-\sin{x}+2$}\\\\
$-\sin{x}+2+\sin{x}+x^2=x^2+2 => x^2+2=x^2+2$\\\\
Therefore $y$ is a solution to $\dfrac{d^2y}{dx^2}+y=x^2+2$.\\\\
Problem 4:\\\\$x=2\cos{t}-3\sin{t}$ \tab{$x''+x=0$}\\\\
$x'=-2\sin{t}-3\cos{t}$ \tab{$x''=-2\cos{t}+3\sin{t}$}\\\\
$2\cos{t}-3\sin{t}-2\cos{t}+3\sin{t}=0 =>0=0 $\\\\
Therefore $x$ is a solution to $x''+x=0$ is a solution.\\\\
Problem 5:\\\\$\theta=2e^{3t}-e^{2t}$ \tab{$\dfrac{d^2\theta}{dt^2}-\theta\dfrac{d\theta}{dt}+3\theta=-2e^{2t}$}\\\\
$\theta'=6e^{3t}-2e^{2t}$ \tab{$\theta''=18e^{3t}-4e^{2t}$}\\\\
$18e^{3t}-4e^{2t}-(2e^{3t}-e^{2t})(6e^{3t}-2e^{2t})+6e^{3t}-3e^{2t}=-2e^{2t}$\\\\
$24e^{3t}-7e^{2t}-12e^{6t}+10e^{5t}-2e^{4t}\neq-2e^{2t}$\\\\
Therefore $\theta$ is  not a solution to $\dfrac{d^2\theta}{dt^2}-\theta\dfrac{d\theta}{dt}+3\theta=-2e^{2t}$\\\\
Problem 6:\\\\$x=\cos{2t}$ \tab{$\dfrac{dx}{dt}+tx=\sin{2t}$}\\\\
$x'=-2\sin{2t}$\\\\
$-2\sin{2t}+t\cos{2t}=\sin{2t} => t\cos{2t}\neq3\sin{2t}$\\\\
Therefore $x$ is not a solution to $\dfrac{dx}{dt}+tx=\sin{2t}$.\\\\\\\\
Problem 9:\\\\
$x^2+y^2=4$ \tab{$\dfrac{dy}{dx}=\dfrac{x}{y}$}\\\\
\\$2x+2yy'=0=>2yy'=-2x=>y'=-\dfrac{x}{y}$\\\\
$-\dfrac{x}{y}\neq\dfrac{x}{y}$\\\\
Therefore $x^2+y^2=4$ is not a solution to $\dfrac{dy}{dx}=\dfrac{x}{y}$.\\\\
Problem 10:\\\\
$y-\ln{y}=x^2+1$ \tab{$\dfrac{dy}{dx}=\dfrac{2xy}{y-1}$}\\\\
\\$y'-\dfrac{y'}{y}=2x=>y'\left(1-\dfrac{1}{y}\right)=2x=>y'=\dfrac{2xy}{y-1}$\\\\
\\Therefore $y-\ln{y}=x^2+1$ is a solution to $\dfrac{dy}{dx}=\dfrac{2xy}{y-1}$.\\\\
Problem 22:\\\\
$\phi(x)=c_1e^x+c_2e^{-2x}$\tab{$\dfrac{d^2y}{dx^2}+\dfrac{dy}{dx}-2y=0$}\\\\
$y=c_1e^x+c_2e^{-2x}$\\
$y'=c_1e^x-2c_2e^{-2x}$\\
$y''=c_1e^x+4c_2e^{-2x}$\\\\
$c_1e^x+4c_2e^{-2x}+c_1e^x-2c_2e^{-2x}-2(c_1e^x+c_2e^{-2x})=0$\\
All values cancel making $0=0$ therefore $\phi$ is a solution.\\\\
Find $c_1$ and $c_2$ such that the initial conditions are met.\\\\
a) $y(0)=2$, $y'(0)=1$\\\\
After plugging in 0 into x need to find constant values such that,\\\\
$c_1+c_2=2$\\
$c_1-2c_2=1$\\
$c_1+4c_2=3$ (get this one by plugging initial conditions into the ODE)\\\\\\\\
Using a bit of linear algebra and row reductions I came to the following matrix
\begin{center}$\begin{bmatrix}
1 & 0 & \dfrac{5}{3}\\\\
0 & 1 & \dfrac{1}{3}\\\\
0 & 0 & 0
\end{bmatrix}$\end{center}
This tells us that $c_1=\dfrac{5}{3}$ and $c_2=\dfrac{1}{3}$\\\\
b) $y(1)=1$, $y'(1)=0$\\\\
Using the same idea as letter (a) we need to find constants such that,\\\\
$ec_1+\dfrac{c_2}{e^2}=1$\\
$ec_1-\dfrac{2c_2}{e^2}=0$\\
$ec_1+\dfrac{4c_2}{e^2}=2$\\\\
Use linear algebra again and come to a reduced matrix
\begin{center}$\begin{bmatrix}
1 & 0 & \dfrac{2}{3e}\\\\
0 & 1 & \dfrac{e^2}{3}\\\\
0 & 0 & 0
\end{bmatrix}$\end{center}
The matrix indicates that $c_1=\dfrac{2}{3e}$ and $c_2=\dfrac{e^2}{3}$
\end{document}
