\documentclass[12pt]{exam}
\usepackage[utf8]{inputenc}
\usepackage{amsmath,mathtools,amssymb}

\title{\textbf{MATH 311 Homework 4.1}}
\author{Will Townsend}
\date{April 08, 2022}

\begin{document}

\maketitle

\section*{Problem 1}
$y=c_1+c_2\cos{x}+c_3\sin{x};\qquad y(\pi)=0,\quad y'(\pi)=2,\quad y''(\pi)=1$\\\\
$1=-c_2\cos{\pi}-c_3\sin{\pi}=>c_2=1$\\
$2=-c_2\sin{\pi}+c_3\cos{\pi}=>c_3=-2$\\
$0=c_1+c_2\cos{\pi}+c_3\sin{\pi}=>0=c_1+1\cos{\pi}-2\sin{\pi}=>0=c_1-1=>c_1=1$\\\\
$y=1+\cos{x}-2\sin{x}$
\section*{Problem 2}
$y^{(4)}+y''=0$\\\\
W=\begin{vmatrix}$
    1 & x & \sin{x} & \cos{x}\\
    0 & 1 & \cos{x} & -\sin{x}\\
    0 & 0 & -\sin{x} & -\cos{x}\\
    0 & 0 & -\cos{x} & \sin{x}$
\end{vmatrix} =
\begin{vmatrix}$
    1 & \cos{x} & -\sin{x}\\
    0 & -\sin{x} & -\cos{x}\\
    0 & -\cos{x} & \sin{x}$
\end{vmatrix} =
\begin{vmatrix}$
    -\sin{x} & -\cos{x}\\
    -\cos{x} & \sin{x}$
\end{vmatrix} =\begin{center} $-\sin^2{x}-\cos^2{x}=-1\neq0\therefore$\\ the set is linearly independent.\end{center}\\
$1,\quad 0+0=0=>0=0\:\checkmark$\\
$x,\quad 0+0=0=>0=0\:\checkmark$\\
$\sin{x},\quad\sin{x}-\sin{x}=0=>0=0\:\checkmark$\\
$\cos{x},\quad\cos{x}-\cos{x}=0=>0=0\:\checkmark$\\
Therefore the functions form a Fundamental set of solutions for the DE.\\
General Solution: $y=c_1+c_2x+c_3\sin{x}+c_4\cos{x}$
\pagebreak
\section*{Problem 3}
$y''+9y=0\qquad y_1=\sin{3x}$\\\\
$y_2=u\cdot\sin{3x}\qquad y_2'=u'\sin{3x}+3u\cos{3x}\qquad y_2''=u''\sin{3x}+6u'\cos{3x}-9u\sin{3x}$\\\\
$u''\sin{3x}+6u'\cos{3x}-9u\sin{3x}+9u\sin{3x}=0\qquad w=u'$\\\\
$\int\dfrac{dw}{w}=\int\dfrac{6\sin{3x}}{\cos{3x}}dx=>\ln{w}=\ln{u^{-2}}=>w=\dfrac{1}{\sin^2{3x}}=> \int w=\int\csc^2{3x}\\\\u=-\frac{1}{3}\cot{3x}\therefore$\\\\
$y_2=-\frac{1}{3}\cot{3x}\cdot\sin{3x}=\cos{3x}$\\
General Solution: $y=c_1\sin{3x}+c_2\cos{3x}$
\section*{Problem 4}
$x^2y''+2xy'-6y=0,\qquad y_1=x^2$\\
$y_2=ux^2\qquad y_2'=u'x^2+2ux\qquad y_2''=u''x^2+4u'x+2u$\\\\
$u''x^4+4u'x^3+2ux^2+2u'x^3+4ux^2-6ux^2=0=>u''x^4+6u'x^3=0\quad w=u'$\\\\
$\dfrac{dw}{dx}+\dfrac{6w}{x}=0\:(I(x)=x^6)=>\int(x^6w)'=\int0=>w=x^{-6}=>u=x^{-5}$\\\\
$y_2=x^{-5}x^2=x^{-3}$\\
General Solution: $y=c_1x^2+c_2x^{-3}$
\end{document}
